src/ReadOnlyFS.v
@@ -364,26 +364,6 @@ Proof.
   intuition eauto.
 Qed.
 
-Theorem ret_ok : forall Sigma (delta: Protocol Sigma) T (v: T),
-    SPEC delta, tid |-
-             {{ (_:unit),
-              | PRE d hm m s_i s: True
-              | POST d' hm' m' s_i' s' r:
-                  r = v /\
-                  d' = d /\
-                  hm' = hm /\
-                  m' = m /\
-                  s_i' = s_i /\
-                  s' = s
-             }} Ret v.
-Proof.
-  intros.
-  CoopConcurMonad.monad_simpl.
-  eapply valid_unfold; intros.
-  deex.
-  eapply H1 in H0; intuition eauto.
-Qed.
-
 Instance rely_preorder Sigma (delta: Protocol Sigma) tid : PreOrder (rely delta tid).
 Proof.
   unfold rely; constructor; hnf; intros; eauto.
